Cslib/Computability/Machines/MultiTapeTuring/UniversalTM.lean
@@ -19,6 +19,8 @@ namespace Turing
 
 namespace UniversalTM
 
+open Routines
+
 /-- TODO document -/
 public abbrev Var := ℕ
 
@@ -31,31 +33,77 @@ public structure TapeCell where
 
 /-- Cells from `k` Turing tapes combined into one cell. -/
 public structure MultiCell (k : ℕ) where
-  /-- TODO document -/
+  /-- One cell from each tape. -/
   cells : Vector TapeCell k
-  /-- TODO document -/
+  /-- Is this the left-most cell (across all tapes)? -/
   isLeftEnd : Bool
-  /-- TODO document -/
+  /-- Is this the right-most cell (across all tapes)? -/
   isRightEnd : Bool
 
 public instance : StrEnc TapeCell where
-  toData cell := Data.list [StrEnc.toData cell.c, StrEnc.toData cell.containsHead]
-  fromData
-    | Data.list [c, containsHead] => do
-        pure { c := ← StrEnc.fromData c, containsHead := ← StrEnc.fromData containsHead }
-    | _ => none
+  toData cell := StrEnc.toData (cell.c, cell.containsHead)
+  fromData d := do
+    let (c, containsHead) ← StrEnc.fromData d
+    pure { c, containsHead }
   fromData_toData := by
     intro c
-    sorry
+    simp
 
-/- Layout of the tapes:
-Tape 1: Encoding of the tapes
-Tape 2: current state
-Tape 3: builds up input for transition function and stores output of transition function
+public instance (α : Type) [StrEnc α] (k : ℕ) : StrEnc (Vector α k) where
+  toData v := StrEnc.toData v.toList
+  fromData d := do
+      let ls : List α ← StrEnc.fromData d
+      if h : ls.length = k then
+        pure ⟨ls.toArray, h⟩
+      else
+        none
+  fromData_toData := by
+    intro v
+    simp [Vector.toList]
+
+public instance : StrEnc (MultiCell (k : ℕ)) where
+  toData mc := StrEnc.toData (mc.cells, mc.isLeftEnd, mc.isRightEnd)
+  fromData d := do
+    let (cells, isLeftEnd, isRightEnd) <- StrEnc.fromData d
+    pure { cells, isLeftEnd, isRightEnd }
+  fromData_toData := by
+    intro v
+    simp
+
+/-
+Outline of UTM:
+while the current state is not None:
+- for each tape, find the head position on the multi-tape and copy the current symbol to an aux tape.
+- now the aux tape contains the symbols in the correct order.
+- copy the current state to the aux tape.
+- the contents of the aux tape is exactly the input to the transition function
+- "evaluate the transition function" by iterating through its table and storing the result on another tape
+- execute the actions for each of the tapes:
+  - find the head. update the symbol, update the head marking according to the move action
+    (potentially extend the tape to the left or right)
+- update the current state
 -/
 
--- def findTapeSymbol (k : ℕ) (tapes : Fin k → BiTape Char) (i : Fin k) : TapeCell :=
---   { c := (tapes i).head, containsHead := true }
+/- sub-routines we need:
+- move to the first element of a list that satisfies a condition:
+  tm₁ tm₂ tm₃: For each item in the list: if tm₁ outputs true on an aux tape, run tm₂.
+  if it never outputs true, run tm₃
+- evaluate a function given by a list of input-output pairs
+- update an element in a list, whose encoding size must be the same
+- extend a list to the right
+-/
+
+/-- The encoding of the given tapes as a list of `MultiCell`s. -/
+def encodeTapes (k : ℕ) (tapes : Fin k → BiTape Char) (shifts : Fin k → ℤ) : List (MultiCell k) :=
+  sorry
+
+def getHeadSymbol (k : ℕ) (tapeIdx : ℕ) (mt out aux : Fin k) : MultiTapeTM k Char :=
+  -- Find the cell where the tapeIdx-th tape has the head
+  find_list mt aux (at_path [0, tapeIdx, 1] mt (copyEnc mt aux))
+    -- copy the symbol to out
+    (at_path [0, tapeIdx, 0] mt (copy_to_list mt out))
+    -- otherwise do nothing (because we know there is a head marker)
+    (noop)
 
 
 
